% ===============================
% Worksheet / Manual Template
% ===============================
\documentclass[12pt, a4paper]{article}

% ===============================
% Metadata
% ===============================
\newcommand*{\CourseCode}{MAT221}
\newcommand*{\CourseTitle}{Complex Variables \& Laplace Transform}
\newcommand*{\Chapter}{Complex Functions}
\newcommand*{\Topics}{Exponential, Logarithmic, Circular and Hyperbolic Functions}
\newcommand*{\DocDate}{October 22, 2025}

\include{header.tex}

% ==========================================
% Document
% ==========================================
\begin{document}
\FrontPage
\Large

\begin{heading}
	Single valued and multi valued functions
\end{heading}

\begin{definition}[Single-valued Function]
	A function \( f: D \to \C \) is called single-valued if for every input \( z \in D \), there is exactly one output \( w \in \C \) such that \( f(z) = w \).
\end{definition}

\vfill

\begin{definition}[Multi-valued Function]
	A function \( f: D \to \mathcal{P}(\C) \) is called multi-valued if for some input \( z \in D \), there are multiple outputs \( w_1, w_2, \ldots, w_n \in \C \) such that \( f(z) = \{w_1, w_2, \ldots, w_n\} \) with \( n > 1 \).\\[8pt]

	A multiple-valued function can be considered as a collection of single-valued functions, each member of which is called a branch of the function.
\end{definition}

\vfill

\clearpage

\begin{heading}
	Why some functions are multi-valued?
\end{heading}

\clearpage

\begin{heading}
	The Exponential Function
\end{heading}

\clearpage

\begin{theorem}[Complex Exponential Function is Periodic]
	The complex exponential function \( e^z \) is periodic with period \( 2\pi i \).
\end{theorem}

\clearpage

\begin{problem}
	Find all values of \( z \in \C \) such that \[e^z = -1 + i\sqrt{3}.\]
\end{problem}

\clearpage

\begin{problem}
	Find all values of \( z \in \C \) such that \[e^{4z} = -1\]
\end{problem}

\clearpage

\begin{heading}
	The Logarithmic Function
\end{heading}

\clearpage

\begin{definition}[Complex Logarithm]
	The complex logarithm of a non-zero complex number \( z \) is defined as \[\log z = \ln|z| + i\arg z\] where \( \arg z \) is the argument of \( z \).\\[15pt]
	Note: The complex logarithm is a multi-valued function due to the multi-valued nature of the argument \( \arg z \).
\end{definition}

\clearpage

\begin{problem}
Show that:

\begin{enumerate}[label=(\roman*)]
    \item \(\ln(-1 + \sqrt{3}i) = \ln 2 + 2\left(n + \tfrac{1}{3}\right)\pi i\)
    
    \item \(\ln(1 - i) = \tfrac{1}{2}\ln 2 + \left(2n + \tfrac{7}{4}\right)\pi i\)
    
    \item \(\ln(i^{1/2}) = \left(n + \tfrac{1}{4}\right)\pi i\)
\end{enumerate}
\end{problem}

\clearpage

\begin{heading}
	Circular Functions
\end{heading}

\vspace{10pt}

\begin{definition}[Complex Sine and Cosine Functions]
	The complex sine and cosine functions are defined as follows:
	\[
	\sin z = \frac{e^{iz} - e^{-iz}}{2i}, \quad \cos z = \frac{e^{iz} + e^{-iz}}{2}
	\]
	for all \( z \in \C \).
\end{definition}

\clearpage

\begin{heading}
	Inverse Circular Functions
\end{heading}

\vspace{10pt}

\begin{definition}[Inverse Circular Functions]
	The inverse circular functions for complex numbers are defined as follows:
	\begin{align*}
	\sin^{-1} z &= -i \ln\left(iz + \sqrt{1 - z^2}\right) \\[6pt]
	\cos^{-1} z &= -i \ln\left(z + \sqrt{z^2 - 1}\right) \\[6pt]
	\tan^{-1} z &= \frac{i}{2} \ln\left(\frac{i + z}{i - z}\right) \\[6pt]
	\cot^{-1} z &= \frac{i}{2} \ln\left(\frac{z - i}{z + i}\right) \\[6pt]
	\sec^{-1} z &= -i \ln\left(\frac{1 + \sqrt{1 - z^2}}{z}\right) \\[6pt]
	\cosec^{-1} z &= -i \ln\left(\frac{i + \sqrt{z^2 - 1}}{z}\right)
	\end{align*}
	for all \( z \in \C \).
\end{definition}

\clearpage

\begin{problem}
	Prove that for all \( z \in \C \):
	\[\sin^{-1} z = -i \ln\left(iz + \sqrt{1 - z^2}\right)\]
\end{problem}

\clearpage

\begin{problem}
	Prove that for all \( z \in \C \):
	\[\sec^{-1} z = -i \ln\left(\frac{1 + \sqrt{1 - z^2}}{z}\right)\]
\end{problem}

\clearpage

\begin{problem}
	Prove that for all \( z \in \C \):
	\[\cot^{-1} z = \frac{i}{2} \ln\left(\frac{z - i}{z + i}\right)\]
\end{problem}

\clearpage

\begin{problem}
	Solve for \( z \in \C \):
	\[\sin z = 2\]
\end{problem}

\clearpage

\begin{heading}
	Hyperbolic Functions
\end{heading}

\vspace{10pt}

\begin{definition}[Sine Hyperbolic and Cosine Hyperbolic Functions]
	The complex sine and cosine functions are defined as follows:
	\[
	\sinh z = \frac{e^{z} - e^{-z}}{2}, \quad \cosh z = \frac{e^{z} + e^{-z}}{2}
	\]	
	for all \( z \in \C \).
\end{definition}

\clearpage

\begin{heading}
	Inverse Hyperbolic Functions
\end{heading}

\vspace{10pt}

\begin{definition}[Inverse Hyperbolic Functions]
The inverse hyperbolic functions for complex numbers are defined as follows:
\[
\begin{aligned}
\sinh^{-1} z &= \ln\left(z + \sqrt{z^2 + 1}\right) \\[6pt]
\cosh^{-1} z &= \ln\left(z + \sqrt{z^2 - 1}\right) \\[6pt]
\tanh^{-1} z &= \frac{1}{2} \ln\left(\frac{1 + z}{1 - z}\right) \\[6pt]
\coth^{-1} z &= \frac{1}{2} \ln\left(\frac{z + 1}{z - 1}\right) \\[6pt]
\sech^{-1} z &= \ln\left(\frac{1 + \sqrt{1 - z^2}}{z}\right)\\[6pt]
\cosech^{-1} z &= \ln\left(\frac{1 + \sqrt{1 + z^2}}{z}\right)
\end{aligned}
\]
for all \( z \in \C \).
\end{definition}

\clearpage

\begin{problem}
	Prove that for all \( z \in \C \):
	\[\cosh^{-1} z = \log\left(z + \sqrt{z^2 - 1}\right)\]
\end{problem}

\clearpage

\begin{problem}
	Prove that for all \( z \in \C \):
	\[\cosech^{-1} z = \ln\left(\frac{1 + \sqrt{1 + z^2}}{z}\right)\]
\end{problem}

\clearpage

\begin{problem}
	Prove that for all \( z \in \C \):
	\[\tanh^{-1} z = \frac{1}{2} \log\left(\frac{1 + z}{1 - z}\right)\]
\end{problem}

\clearpage

\begin{problem}
	Solve for \( z \in \C \):
	\[\cosh z = 3i\]
\end{problem}

\clearpage

\begin{heading}
	Properties of Circular and Hyperbolic Functions
\end{heading}

\vspace{10pt}

\begin{theorem}
For all \( z \in \C \):
\[\sin z = \sin x \cosh y + i \cos x \sinh y\]
\[\cos z = \cos x \cosh y - i \sin x \sinh y\]
where \( z = x + iy \), \( x, y \in \R \).
\end{theorem}

\vspace{10pt}

\begin{theorem}
For all \( z \in \C \):
\[\sinh z = \sinh x \cos y + i \cosh x \sin y\]
\[\cosh z = \cosh x \cos y + i \sinh x \sin y\]
where \( z = x + iy \), \( x, y \in \R \).
\end{theorem}

\vspace{10pt}

\begin{theorem}
For all \( z \in \C \):
\begin{align*}
\sin(iz) &= i\sinh z, \\[4pt]
\cos(iz) &= \cosh z, \\[4pt]
\sinh(iz) &= i\sin z, \\[4pt]
\cosh(iz) &= \cos z.
\end{align*}
\end{theorem}

\clearpage

\begin{theorem}
For all \( z \in \C \):
\[\\cos^2 z + \sin^2 z = 1\]
\[cosh^2 z - sinh^2 z = 1\]
\end{theorem}

\vspace{10pt}

\begin{theorem}
For all \( z \in \C \):
\[\frac{d}{dz}(\sin z) = \cos z, \quad \frac{d}{dz}(\cos z) = -\sin z\]
\[\frac{d}{dz}(\sinh z) = \cosh z, \quad \frac{d}{dz}(\cosh z) = \sinh z\]
\end{theorem}



\EndPage
\end{document}